codes/PTSExample.v
@@ -1,0 +1,96 @@
+Require Import List.
+Import ListNotations.
+
+Require Import Thesis.PTSSignature.
+Require Import Thesis.PTS.
+
+Module PTSExampleSig <: PTS_SIGNATURE.
+
+Inductive ex_sort :=
+  | Star
+  | Box.
+
+Definition Sort := ex_sort.
+
+Inductive ex_A : Sort -> Sort -> Prop :=
+    | ax_star : ex_A Star Box.
+
+Definition A := ex_A.
+
+Inductive ex_R : Sort -> Sort -> Sort -> Prop :=
+    | rule_star : ex_R Star Star Star
+    | rule_box : ex_R Box Box Box.
+
+Definition R := ex_R.
+
+End PTSExampleSig.
+
+
+Module PTSExample := PTS(PTSExampleSig).
+
+Import PTSExample.
+Import PTSExampleSig.
+
+Check typing.
+
+Definition star : term :=
+  t_sort Star.
+
+Definition box : term :=
+  t_sort Box.
+
+
+Example star_typing :
+  [] ⊢ star ∈ box.
+Proof.
+    unfold star, box.
+    apply typing_axiom.
+    apply ax_star.
+Qed.
+
+Definition x : var :=
+  {| var_sort := Box;
+     var_idx := 0 |}.
+
+Definition y : var :=
+  {| var_sort := Box;
+     var_idx := 1 |}.
+
+Example typingE1:
+    [] ⊢ 
+    (t_lam x star (t_lam y star (t_var x)))
+    ∈
+    (t_pi x star (t_pi y star star)).
+Proof.
+    unfold star.
+    apply typing_lam with (s' := Box).
+
+    - apply typing_lam with (s' := Box).
+
+        + apply typing_weak with (x := y) (B := t_sort Star) (s := Box).
+          * simpl. unfold is_fresh. simpl. destruct (eq_var_dec y x).
+            ** discriminate.
+            ** reflexivity.
+          * reflexivity.
+          * apply typing_var with (s := Box).
+            ** reflexivity.
+            ** reflexivity.
+            ** apply typing_axiom. apply ax_star.
+          * apply typing_axiom. apply ax_star.
+        
+        + apply typing_pi with (s1 := Box) (s2 := Box).
+          * reflexivity.
+          * apply typing_axiom. apply ax_star.
+          * apply typing_axiom. apply ax_star.
+          * apply rule_box.
+
+    - apply typing_pi with (s1 := Box) (s2 := Box).
+      + reflexivity.
+      + apply typing_axiom. apply ax_star.
+      + apply typing_pi with (s1 := Box) (s2 := Box).
+        * reflexivity.
+        * apply typing_axiom. apply ax_star.
+        * apply typing_axiom. apply ax_star.
+        * apply rule_box.
+      + apply rule_box.
+Qed.
